:wrench: complete part1

part1.dfy
@@ -2,12 +2,305 @@
     Part 1: Mini exercises
 
     A. Writing specifications
+
+    Consider the following function:
+*/
+
+function max(x: int, y: int): int
+{
+  if x > y then x else y
+}
+
+/*
+    Write specifications for the following properties of max using Dafny.
+    For each property, you should fill in the Test method
+    with an assertion that demonstrates the property.
+    If the test does not pass (Dafny doesn't show a green line), comment out
+    only the assertion line (but leave the Test method there).
+
+    1. The maximum of a number with itself is the same number.
+    2. The maximum of x and y is the same as the maximum of y and x.
+    3. Addition distributes over max:
+       max(x, y) + z is the same as max(x + z, y + z).
+    4. Multiplication distributes over max:
+       max(x, y) * z is the same as max(x * z, y * z).
+    5. Max distributes over addition:
+       max(x, y + z) is equal to the sum of max(x, y) and max(x, z).
+    6. The maximum of x and -x is always equal to the absolute value of x.
+       You will need to define the abs function for this property.
+    7. If x is positive (greater than zero), then max(x, y) is also positive.
+       To test this property, use a precondition on TestMax7 instead
+       of just a plain assertion.
+*/
+
+method TestMax1(x: int)
+{
+  assert max(x, x) == x;
+}
+
+method TestMax2(x: int, y: int)
+{
+  // TODO
+}
+
+method TestMax3(x: int, y: int, z: int)
+{
+  // TODO
+}
+
+method TestMax4(x: int, y: int, z: int)
+{
+  // TODO
+}
+
+method TestMax5(x: int, y: int, z: int)
+{
+  // TODO
+}
+
+method TestMax6(x: int)
+{
+  // TODO
+}
+
+method TestMax7(x : int, y: int)
+  // requires ...
+{
+  // TODO
+}
+
+/*
+    8. Use the Dafny "show counterexample" feature to find a counterexample
+    to all the properties that are not true:
+
+    - Uncomment all the assertions that are not true
+    - Right click, Dafny --> "Show counterexample (experimental)"
+    - Right click, Dafny --> "Copy counterexamples to clipboard"
+
+    Copy paste the output below.
+    Make sure to comment out the assertions again after you are done.
+
+    ###### Answer Q8 ######
+
+    ###### End of Answer ######
 */
 
 /*
-    B. TODO
+    B. Abstraction and interfaces
+
+    This problem explores the concept of abstraction and interfaces
+    through a binary search program.
+
+    Many times in programming, there are multiple ways to implement
+    a procedure or data structure -- as long as it satisfies the
+    *interface* that we are expecting (pre and post conditions),
+    it doesn't matter what the implementation of the procedure is.
+
+    We begin with a between(a, b) function that should return
+    a value between a and b.
+
+    9. The between function requires a precondition in order to
+    implement it. Implement the precondition to between
+    in the function between_precond.
+    Your precondition should be the weakest possible precondition
+    (the weakest possible condition on a and b) that makes it possible
+    to impleemnt the following function in Q9.
+*/
+
+function between_precond(a: int, b: int): bool
+{
+  // TODO: replace with weakest possible precondition
+  false
+}
+
+/*
+  10. Implement the "between" function in three different ways.
+
+  Make sure you don't modify the function signature
+  or pre/postconditions for any of the versions.
+*/
+
+method between_v1(a: int, b: int) returns (result: int)
+  requires between_precond(a, b)
+  ensures a < result && result < b
+{
+  // TODO
+}
+
+method between_v2(a: int, b: int) returns (result: int)
+  requires between_precond(a, b)
+  ensures a < result && result < b
+{
+  // TODO
+}
+
+method between_v3(a: int, b: int) returns (result: int)
+  requires between_precond(a, b)
+  ensures a < result && result < b
+{
+  // TODO
+}
+
+/*
+  11. Use your between function to implement
+  and prove a binary search algorithm.
+
+  Requirements:
+
+  - This binary search algorithm takes as input
+    a function on integers, f, which is assumed
+    to be monotonically increasing:
+      for all x, y: int :: x < y ==> f(x) <= f(y)
+
+  - The binary search algorithm should return
+    the smallest value x such that
+      f(x) >= target.
+    The postcondition is written so that you will
+    need to prove this!
+
+  - Don't modify the function signature or
+    pre/postconditions to binary_search.
+
+  - Your function should call between_v1, between_v2,
+    or between_v3 at least once.
+*/
+
+method binary_search(
+  f: int -> int,
+  min_val: int,
+  max_val: int,
+  target: int
+) returns (result: int)
+  // Precondition: `f` is monotonically increasing and passes
+  // `target` somewhere between `min_val` and `max_val`
+  requires forall x, y :: x < y ==> f(x) <= f(y)
+  requires min_val < max_val
+  requires f(min_val) < target
+  requires f(max_val) >= target
+  // Postcondition: result is the smallest x such that f(x) >= target
+  ensures f(result) >= target
+  ensures forall x :: x < result ==> f(x) < target
+  // Remove the following line to implement
+  requires false
+{
+  // TODO
+}
+
+/*
+  12. Uncomment the following tests to check whether your
+  implementation of binary_search is working as expected.
+*/
+
+function double(x: int): int
+{
+  x * 2
+}
+
+// TODO: Uncomment
+// method TestBinarySearch1()
+// {
+//   var result1 := binary_search(double, 0, 10, 4);
+//   var result2 := binary_search(double, 0, 10, 5);
+//   var result3 := binary_search(double, 0, 10, 20);
+//   assert result1 == 2;
+//   assert result2 == 3;
+//   assert result3 == 10;
+// }
+
+function square(x: int): int
+{
+  x * x
+}
+
+// TODO: Uncomment
+// method TestBinarySearch2()
+// {
+//   var result1 := binary_search(square, 0, 10, 10);
+//   var result2 := binary_search(square, 0, 10, 16);
+//   var result3 := binary_search(square, 0, 10, 100);
+//   assert result1 == 4;
+//   assert result2 == 4;
+//   assert result3 == 10;
+// }
+
+/*
+  13. Try replacing between_v1, between_v2, or between_v3 in
+  the implementation of binary_search. What happens?
+
+  Are there advantages of leaving the interface (pre/postconditions)
+  for between abstract so that multiple implementations are possible?
+
+  ###### Answer Q13 ######
+
+  ###### End of Answer ######
+
+  14. Which of your between functions is the most efficient?
+  Which one would be the best to use in the binary search algorithm?
+
+  ###### Answer Q14 ######
+
+  ###### End of Answer ######
 */
 
 /*
-    C. TODO
+  C. Strongest postconditions and weakest preconditions
+
+  Recall that on HW1 you were asked to write specs that
+  "should completely describe the behavior of the function
+  on all possible inputs."
+  The underlying concept is that of *strongest postconditions*
+  and (in the opposite directino), *weakest preconditions*.
+
+  Use the methods we discussed in class to find the strongest
+  postcondition and weakest precondition for each statement by adding
+  an assert() statement after every line of code in the function.
+
+  15. split_in_half
+  (strongest postcondition)
+
+  16. pad_with_spaces
+  (weakest precondition)
+*/
+
+method SplitInHalf(s: string) returns (result1: string, result2: string)
+  requires true
+  // ensures ... // fill in after finding the strongest postcondition
+{
+  var mid := (|s| + 1) / 2;
+  if mid == 0 {
+    result1 := "";
+    result2 := "";
+  } else {
+    result1 := s[..(mid - 1)];
+    result2 := s[mid..];
+  }
+}
+
+method PadWithSpaces(s: string, n: int) returns (result: string)
+  requires false // remove this line to work on this part!
+  // requires ... // fill in after finding the weakest precondition
+  ensures |result| == n
+  ensures n >= |s|
+  ensures result[..|s|] == s
+  ensures forall i :: |s| <= i < n ==> result[i] == ' '
+{
+  var prefix := s;
+  var padding := seq(n - |s|, i => ' ');
+  result := prefix + padding;
+}
+
+/*
+  17. What precondition fell out of the weakest precondition calculation?
+  Compare with the implementation we saw in Python:
+
+  def pad_with_spaces(s, n):
+      if len(s) > n:
+          return None
+      return s + " " * (n - len(s))
+
+  Do you see advantages to this version of the function above in Dafny?
+
+  ###### Answer Q17 ######
+
+  ###### End of Answer ######
 */
